{
  "@context": {
    "rdf": "http://www.w3.org/1999/02/22-rdf-syntax-ns#",
    "rdfs": "http://www.w3.org/2000/01/rdf-schema#",
    "xsd": "http://www.w3.org/2001/XMLSchema#",
    "dc": "http://purl.org/dc/elements/1.1/",
    "s": "http://schema.org/",
    "@vocab": "http://schema.howarddierking.com/",
    "@base": "http://schema.howarddierking.com/"
  },
  "@graph": [
    {
      "@id": "/Bug",
      "@type": "rdfs:Class",
      "rdfs:label": "Bug",
      "rdfs:comment": "A unit of work. Traditionally tied to a failure in a software application."
    },
    {
      "@id": "/title",
      "@type": "rdf:Property",
      "rdfs:label": "title",
      "rdfs:comment": "The name of the item.",
      "s:rangeIncludes": [
        { "@id": "s:Text" }
      ],
      "s:domainIncludes": [
        { "@id": "/Bug" }
      ]
    },
    {
      "@id": "/status",
      "@type": "rdf:Property",
      "rdfs:label": "status",
      "rdfs:comment": "An identifier describing the state of an object in a workflow.",
      "s:rangeIncludes": [
        { "@id": "s:Text" }
      ],
      "s:domainIncludes": [
        { "@id": "/Bug" }
      ]
    },
    {
      "@id": "/description",
      "@type": "rdf:Property",
      "rdfs:label": "description",
      "rdfs:comment": "A more detailed explanation than what may be contained in an ojbect's name.",
      "s:rangeIncludes": [
        { "@id": "s:Text" }
      ],
      "s:domainIncludes": [
        { "@id": "/Bug" }
      ]
    },
    {
      "@id": "/assignedTo",
      "@type": "rdf:Property",
      "rdfs:label": "assignedTo",
      "rdfs:comment": "Zero or more agents that are assigned to a unit of work.",
      "s:rangeIncludes": [
        { "@id": "/Collaborator" }
      ],
      "s:domainIncludes": [
        { "@id": "/Bug" }
      ]
    },
    {
      "@id": "/watchedBy",
      "@type": "rdf:Property",
      "rdfs:label": "watchedBy",
      "rdfs:comment": "Zero or more agents that wish to be kept updated on the status of a unit of work.",
      "s:rangeIncludes": [
        { "@id": "/Collaborator" }
      ],
      "s:domainIncludes": [
        { "@id": "/Bug" }
      ]
    }
  ]
}
